entry_point diagram proven for half of the phases

backend/Cminor.v
@@ -609,12 +609,13 @@ Inductive initial_state (p: program): state -> Prop :=
       initial_state p (Callstate f nil Kstop m0).
 
 Inductive entry_point (p: program): mem -> state -> val -> list val -> Prop :=
-  | entry_point_intro: forall b f m0 fp arg,
+  | entry_point_intro: forall b f m0 fp args,
       let ge := Genv.globalenv p in
-      Genv.find_symbol ge p.(prog_main) = Some b ->
+      Mem.mem_wd m0 ->
+      Mem.arg_well_formed args m0 ->
+      globals_not_fresh ge m0 ->
       Genv.find_funct_ptr ge b = Some f ->
-      funsig f = signature_main ->
-      entry_point p m0 (Callstate f nil Kstop m0) fp arg.
+      entry_point p m0 (Callstate f args Kstop m0) fp args.
 
 (** A final state is a [Returnstate] with an empty continuation. *)
 
@@ -1220,16 +1221,24 @@ Theorem bigstep_semantics_sound:
 Proof.
   constructor;
     intros.
-(* termination *)
+-(* termination *)
   inv H. econstructor; econstructor.
   split. econstructor; eauto.
   econstructor; eauto.
-  split. apply eval_funcall_steps. eauto. red; auto.
+  + eapply Genv.initmem_inject; eauto.
+  + constructor.
+  + unfold globals_not_fresh.
+    erewrite Genv.init_mem_genv_next; eauto; reflexivity.
+  + split. apply eval_funcall_steps. eauto. red; auto.
   econstructor.
-(* divergence *)
+-(* divergence *)
   inv H. econstructor.
   split. econstructor; eauto.
          econstructor; eauto.
+         eapply Genv.initmem_inject; eauto.
+         constructor.
+         unfold globals_not_fresh.
+         erewrite Genv.init_mem_genv_next; eauto; reflexivity.
   eapply forever_plus_forever.
   eapply evalinf_funcall_forever; eauto.
 Qed.
