cfrontend/Csharpminor.v
@@ -532,8 +532,11 @@ Inductive initial_state (p: program): state -> Prop :=
 Inductive entry_point (p: program): mem -> state -> val -> list val -> Prop :=
   | entry_point_intro: forall b f m0 fp args,
       let ge := Genv.globalenv p in
+      Mem.mem_wd m0 ->
+      Mem.arg_well_formed args m0 ->
+      globals_not_fresh ge m0 ->
       Genv.find_funct_ptr ge b = Some f ->
-      entry_point p m0 (Callstate f args Kstop m0) fp args.
+      entry_point p m0 (Callstate f args Kstop m0) fp args. 
 
 (** A final state is a [Returnstate] with an empty continuation. *)
 
