backend/Tailcallproof.v
@@ -582,6 +582,37 @@ Proof.
   constructor. constructor. constructor. apply Mem.extends_refl.
 Qed.
 
+Lemma transf_entry_points:
+   forall (s1 : state) (f : val) (arg : list val) (m0 : mem),
+  entry_point prog m0 s1 f arg ->
+  exists s2 : state, entry_point tprog m0 s2 f arg /\ match_states s1 s2.
+Proof.
+  intros. inv H.
+  exploit funct_ptr_translated; eauto. intro FIND.
+  econstructor; split.
+  
+  - econstructor; eauto.
+    unfold globals_not_fresh.
+    erewrite <- len_defs_genv_next.
+    + unfold ge0 in *. simpl in H2; eapply H2.  
+    + eapply (@match_program_gen_len_defs program); eauto.
+  - econstructor; eauto.
+    + constructor.
+    + clear. induction arg; auto.
+    + apply Mem.extends_refl.
+Qed.
+
+Lemma transf_initial_states':
+  forall s1 : state,
+  Smallstep.initial_state (semantics prog) s1 ->
+  exists s2 : state, Smallstep.initial_state (semantics tprog) s2 /\ match_states s1 s2.
+Proof.
+  eapply (@init_states_from_entry (semantics prog) (semantics tprog));
+    try apply transf_entry_points.
+  - apply (Genv.init_mem_match TRANSL); eauto.
+  - simpl. destruct TRANSL as (P & Q & R). auto.
+Qed.
+  
 Lemma transf_final_states:
   forall st1 st2 r,
   match_states st1 st2 -> final_state st1 r -> final_state st2 r.
@@ -598,7 +629,8 @@ Theorem transf_program_correct:
 Proof.
   eapply forward_simulation_opt with (measure := measure); eauto.
   apply senv_preserved.
-  eexact transf_initial_states.
+  eexact transf_entry_points.
+  eexact transf_initial_states'.
   eexact transf_final_states.
   exact transf_step_correct.
 Qed.
