common/Globalenvs.v
@@ -277,6 +277,8 @@ Qed.
 Definition globalenv (p: program F V) :=
   add_globals (empty_genv p.(prog_public)) p.(prog_defs).
 
+
+
 (** Proof principles *)
 
 Section GLOBALENV_PRINCIPLES.
